In an all incoming momentum framework (the final result is independent of this) we have 4-momentum conservation:

$$\sum\limits_i p^\mu_i=0$$
The [[String/Mandelstam invariants|Mandelstam variables]] are given by:![[String/Mandelstam invariants#^allIncomingPP|Mandelstam variables]]
Thus we have:

$$\begin{align*}
2(s+t+u)&=\sum\limits_{i<j}(p_i+p_j)^2=\sum\limits_{i<j} m_i^2+2p_i^\mu p_{j \mu }+m_j^2\\
&=3\sum\limits_i m_i^2+2\sum\limits_{i<j}p_i^\mu p_{j \mu } 
\end{align*}$$
But from momentum conservation we have:
$$\pqty\Big{\sum\limits_i p_i}^2=\sum\limits_i m_i^2+2\sum\limits_{i<j}p_i^\mu p_{j \mu }\implies 2\sum\limits_{i<j}p_i^\mu p_{j \mu }=-\sum\limits_i m_i^2$$
Plugging back in we have:

$$2(s+t+u)=2\sum\limits_i m_i^2\implies s+t+u=h\qqtext{where} h=\sum\limits_i m_i^2$$
